testdata/cue/comprehensions/default_in_guard.cue
@@ -1,0 +1,9 @@
+staging: bool | *false
+out: {
+	if !staging {
+		prod: true
+	}
+	if staging {
+		dev: true
+	}
+}
